\section*{Problema 2}
Resuelva la ecuaci칩n diferencial en (2) por medio de la transformada de Laplace. 
Su soluci칩n $T(t)$ depender치 de $h$.

\begin{equation}
    T_m(t) = 50 + 20 U(h - t)
\end{equation}
\begin{equation}
    \frac{dT}{dt} = k(T - T_m(t))
\end{equation}

\begin{center}

Sustituyendo (2) en (3),\\
\begin{align*}
    \frac{dT}{dt} = k\bigl(T - 50 - 20U(h - t)\bigr) 
\end{align*}
Con $k = -2\ln{\left(\frac{34}{35}\right)}$ y $T(0) = 85$\\ 
\vspace{12pt}


\textbf{Soluci칩n}\\
\begin{equation*}
    \mathscr{L}\biggl\{\frac{dT}{dt} = kT(t)- 50k - 20kU(t-h)\biggr\}
\end{equation*}

\begin{equation*}
    sT(s) - T(0) = kT(s) - \frac{50k}{s} - \frac{20ke^{-hs}}{s}
\end{equation*}

\begin{equation*}
    (s - k)T(s) = 85 - \frac{50k}{s} - \frac{20ke^{-hs}}{s}
\end{equation*}

\begin{equation*}
    T(t) = \mathscr{L}^{-1} \biggl\{\frac{85}{s-k} - \frac{50k}{s(s-k)} - \frac{20ke^{-hs}}{s(s-k)}\biggr\}
\end{equation*}

\begin{equation*}
    \mathscr{L}^{-1} \biggl\{ \frac{85}{s-k} \biggr\} = 85e^{kt}
\end{equation*} 

\begin{equation*}
    f(t) = \mathscr{L}^{-1} \biggl\{ -\frac{50k}{s(s-k)} \biggr\} = \mathscr{L}^{-1} \biggl\{ \frac{A}{s} + \frac{B}{s-k} \biggr\}
\end{equation*}

$-50k = A(s-k) + B(s)$\\ 
\vspace{8pt}
$A + B = 0$\\ 
\vspace{8pt}
$-A = -50$\\ 
\vspace{8pt}
$A = 50, B = -50$\\ 
\vspace{8pt}

\begin{equation*}
    f(t) = \mathscr{L}^{-1} \biggl\{ \frac{50}{s} - \frac{50}{s-k} \biggr\} = 50 - 50e^{kt}
\end{equation*}

\begin{equation*}
    g(t) = \mathscr{L}^{-1} \biggl\{ -\frac{20ke^{-hs}}{s(s-k)} \biggr\} = \mathscr{L}^{-1} \biggl\{ e^{-hs}\left(-\frac{20k}{s(s-k)}\right) \biggr\} = U(t-h)h(t-h)
\end{equation*}

\begin{equation*}
    g(t-h) = \mathscr{L}_{t-h}^{-1} \biggl\{ -\frac{20k}{s(s-k)} \biggr\} = \mathscr{L}_{t-h}^{-1} \biggl\{ \frac{C}{s} + \frac{D}{s-k} \biggr\}
\end{equation*}

$-20k = C(s-k) + D(s)$\\ 
\vspace{8pt}
$C + D = 0 $\\ 
\vspace{8pt}
$-C = -20$\\ 
\vspace{8pt}
$C = 20, D = -20$

\begin{equation*}
    h(t-h) = \mathscr{L}_{t-h}^{-1} \biggl\{ \frac{20}{s} - \frac{20}{s-k} \biggr\} = 20 - 20e^{k(t-h)}
\end{equation*}

\begin{equation*}
    g(t) = U(t-h)\left( 20 - 20e^{k(t-h)}\right)
\end{equation*}

\begin{equation*}
    T(t) = 85e^{kt} + 50 - 50e^{kt} + U(t-h)\cdot\left( 20 - 20e^{k(t-h)}\right)
\end{equation*}

\begin{equation}
    T(t) = 35e^{kt} + 20U(t-h)\cdot\left( 1 - e^{k(t-h)}\right) + 50; k = -2\ln{\left(\frac{34}{35}\right)}
\end{equation}
\end{center}